DistributedSystems/VerifiedDS/src/Dafny/Distributed/Protocol/CausalMesh/message.dfy
@@ -38,10 +38,10 @@ module CausalMesh_Message_i {
     predicate PacketHasCorrectSrcAndDst(p:Packet)
     {
         match p.msg 
-            case Message_Read(_,_,_) => 0 <= p.src < Clients && 0 <= p.dst < Nodes
-            case Message_Read_Reply(_,_,_,_) => 0 <= p.dst < Clients && 0 <= p.src < Nodes
-            case Message_Write(_,_,_,_) => 0 <= p.src < Clients && 0 <= p.dst < Nodes
-            case Message_Write_Reply(_,_,_) => 0 <= p.dst < Clients && 0 <= p.src < Nodes
+            case Message_Read(_,_,_) => Nodes <= p.src < Nodes + Clients && 0 <= p.dst < Nodes
+            case Message_Read_Reply(_,_,_,_) => Nodes <= p.dst < Nodes + Clients && 0 <= p.src < Nodes
+            case Message_Write(_,_,_,_) => Nodes <= p.src < Nodes + Clients && 0 <= p.dst < Nodes
+            case Message_Write_Reply(_,_,_) => Nodes <= p.dst < Nodes + Clients && 0 <= p.src < Nodes
             case Message_Propagation(_,_,_,_) => 0 <= p.src < Nodes && 0 <= p.dst < Nodes && NodesAreNext(p.src, p.dst)
     }
 }
